still chugging away

Dec5.lean
@@ -6,98 +6,33 @@ namespace Dec5
 -- we're using the subtype notation
 abbrev Vector (α : Type u) (n : Nat) := { l : List α // l.length = n }
 
-theorem enum_from_preserves_items (α : Type u) (n : Nat) (l : List α)
-        : (l.enumFrom n).map Prod.snd = l := by
-  induction l generalizing n with
-  | nil => simp [List.map]
-  | cons hd tl IH => simp [List.enum, List.enumFrom, List.map]
-                     specialize IH (n + 1)
-                     rw [IH]
-                     
-theorem enum_preserves_items (α : Type u) (l : List α) : l.enum.map Prod.snd = l := by
-  simp [List.enum]
-  apply enum_from_preserves_items
-  
-theorem list_map_preserves_length {α β : Type u} (l : List α) (f : α -> β)
-        : (l.map f).length = l.length := by induction l <;> simp
-
-theorem list_enum_preserves_length (α) (l : List α) : l.length = l.enum.length := by
-  simp [List.enum]
-  cases l with
-  | nil => simp [List.enumFrom]
-  | cons hd tl =>
-    simp [List.enumFrom]
-    have f : (List.enumFrom 1 tl).map Prod.snd = tl :=
-      enum_from_preserves_items α 1 tl
-    rw [<- f] simp rw [f]
-    
-theorem enum_bounded {α : Type u} (l : List α) :
-        ∀ x : (Nat × α), x ∈ l.enum -> x.fst < l.length := by
-  intros x p
-  induction l with
-  | nil => contradiction
-  | cons hd tl IH => simp [Membership.mem, List.Mem, List.enum, List.enumFrom] at *
-                     cases x with
-                     | mk i x =>
-                       cases i with
-                       | zero => exact Nat.succ_pos _
-                       | succ i' => sorry
-                       
-#eval [1, 2, 3] |> Utils.enum
-
--- def list_enum_lift {α : Type u} (l : List α) : l.enum -> List (Fin l.length × α)
---   | [] => []
---   | (i, hd) :: tl => (Fin.mk i _, hd) :: list_enum_lift tl
-                              
-                     -- cases x.fst with
-                     -- | zero => exact Nat.succ_pos _
-                     -- | succ n => apply Nat.succ_lt_succ
-
-
 def Vector.nil : Vector α 0 := ⟨[], rfl⟩
 def Vector.cons {α : Type u} (e : α) (v : Vector α n) : Vector α (n + 1) :=
   ⟨e :: v.val, by simp exact v.property⟩
 def Vector.length {α : Type u} (_ : Vector α n) := n
 def Vector.nth {α : Type u} (v : Vector α n) (idx : Fin n) :=
-  let p : idx.val < v.val.length := by
-    have x := v.property
-    rw [x]
-    exact idx.isLt
+  let p : idx.val < v.val.length := by rw [v.property] exact idx.isLt
   v.val[idx.val]'p
 def Vector.set {α : Type u} (v : Vector α n) (idx : Fin n) (el : α) : Vector α n :=
   ⟨ v.val.set idx.val el, by simp exact v.property ⟩
 def Vector.fromList {α} (l : List α) : Vector α l.length := ⟨ l,  rfl ⟩
 
+def Vector.mkSize {α} (default : α) (n : Nat) : Vector α n :=
+  ⟨ Utils.List.mkLength default n, Utils.List.mkLengthCorrect ⟩
+    
+
+-- TODO! fix this definition. how the heck does type equality work?
 def Vector.enum {α} {n} (l : Vector α n) : Vector (Fin n × α) n :=
   -- this is a proof that List (Fin l.length × α) = List (Fin n × a)
-  let l' : List (Fin n × α) := by
-    rw [Eq.symm l.property]
-    exact Utils.enum l.val
-  -- let npr : List.length l.val = n := sorry
-  ⟨
-    l',
-    by simp [Eq.mpr, Eq.subst]
-       have lp : n = List.length (Utils.enum l.val) := sorry
-       rw [ lp]
-  ⟩
-  -- let enumL := l.val.enum
-  -- let l' := enumL.map (λ (i, a) =>
-  --   (Fin.mk i (by simp
-  --                 have pr : (i, a) ∈ List.enum l.val := by
-                    
-  --                 -- have thing := enum_bounded l.val (i, a) pr
-  --                 -- rw [<- l.property]
-  --                 -- exact thing
-  --                 ),
-  --     a))
-  -- ⟨ l' , by simp rw [<- list_enum_preserves_length] exact l.property ⟩
+  let l' : List (Fin n × α) := (Eq.symm l.property) ▸ Utils.enum l.val
+  let p : List.length l' = n := by
+    have leq : l.val.length = l'.length := sorry
+    rw [<- leq]
+    exact l.property
 
--- def Vector.foldlEnum {α β} {n} (f : α -> β -> Fin n -> α) (init : α) (v : Vector β n) : α :=
---   (h f init v).snd
--- where h {α β} {n} (f : α -> β -> Fin n -> α) (init : (Fin n × α)) (v : Vector β n) : (Fin n × α) :=
---   match v with
---   | [] => init
---   | h :: tl => h f init tl
+  ⟨ l', p ⟩
+  
+#eval Vector.enum (Vector.fromList ['a', 'b', 'c'])
 
 notation a ":::" b => Vector.cons a b
 
@@ -106,7 +41,7 @@ structure StackMachine (n : Nat) where
 deriving Repr
   
 def StackMachine.empty : StackMachine 0 :=
-  StackMachine.mk $ Vector.nil
+  StackMachine.mk Vector.nil
   
 def StackMachine.addCol {n : Nat} (sm : StackMachine n) : StackMachine (n + 1) :=
   StackMachine.mk $ sm.stacks.cons []
@@ -131,19 +66,6 @@ def StackMachine.move {n : Nat} (num : Nat) (frm : Fin n) (to : Fin n) (sm : Sta
                | none => sm
     sm'.move n frm to
     
--- #eval StackMachine.empty
---       |> StackMachine.addCol
---       |> StackMachine.addCol
---       |> StackMachine.addCol
---       |> StackMachine.place 0 'Z'
---       |> StackMachine.place 0 'N'
---       |> StackMachine.place 1 'M'
---       |> StackMachine.place 1 'C'
---       |> StackMachine.place 1 'D'
---       |> StackMachine.place 2 'E'
---       |> StackMachine.move 1 1 0
---       |> StackMachine.move 3 0 2
-
 def data : String := "data/dec5.txt"
 
 -- def List.foldl_dep {β} {α : (x : β) -> γ} (f : α → β → α) : (init : α) → List β → α
@@ -165,8 +87,18 @@ def parseStartingMachine (l : List String) : Option ((n : Nat) × StackMachine n
                     match l.length.decEq hd.length with
                     | isTrue p => some $ ⟨ l, p ⟩
                     | isFalse _ => none)
+                    
+  let sm : StackMachine hd.length :=
+    StackMachine.mk (Vector.mkSize [] hd.length)
+    
+  let sm' : StackMachine hd.length :=
+    cleanVecs.foldl
+      (λ acc v =>
+        let v' := v.enum
+        v'.val.foldl (λ acc (p, c) => acc.place p c) acc)
+      sm
                  
-  pure ⟨ hd.length, cleanVecs ⟩
+  pure ⟨ hd.length, sm' ⟩
 
 #eval do (<- Utils.lines data)
       |> List.groupBy (λ (x y : String) =>
