Utils.lean
@@ -19,9 +19,29 @@ def windows (n : Nat) (l : List α) : List (List α) :=
     |> List.map (List.map Prod.snd)
     
 def enum {α} (l : List α) : List (Fin l.length × α) :=
+  help l 0
+  -- match l with
+  -- | [] => []
+  -- | h :: tl => (Fin.mk tl.length (by simp_arith), h) :: (enum tl).map (λ (f, a) => (Fin.succ f, a))
+where help {α} (l : List α) (acc : Fin l.length) : List (Fin l.length × α) :=
   match l with
   | [] => []
-  | h :: tl => (Fin.mk tl.length (by simp_arith), h) :: (enum tl).map (λ (f, a) => (Fin.succ f, a))
+  | hd :: tl => (acc, hd) :: help l (acc.add 1)
+  
+def List.mkLength {α} (default : α) (n : Nat) : List α :=
+  match n with
+  | 0 => []
+  | n+1 => default :: (mkLength default n)
+  
+theorem List.mkLengthCorrect {α} {default : α} {n : Nat} : (List.mkLength default n).length = n := by
+  induction n with
+  | zero => simp [mkLength]
+  | succ n IH => simp [mkLength] exact IH
+  
+theorem enum_preserves_length {α : Type} (l : List α) : l.length = (Utils.enum l).length := by
+  induction l with
+  | nil => simp [enum]
+  | cons hd tl H => simp [enum] exact H
 
 -- match enum tl with
 -- | [] => [(Fin.mk 0 _, h)]
